...

sf/Assignment08_02.v
@@ -10,9 +10,9 @@ Require Export Assignment08_01.
 
 Definition pup_to_n : com :=
   Y ::= ANum 0;;
-  WHILE BNot (BEq (AId Z) (ANum 0)) DO
-    Y ::= APlus (AId Y) (AId Z);;
-    Z ::= AMinus (AId Z) (ANum 1)
+  WHILE BNot (BEq (AId X) (ANum 0)) DO
+    Y ::= APlus (AId Y) (AId X);;
+    Z ::= AMinus (AId X) (ANum 1)
   END.
 
 Example pup_to_2_ceval :
@@ -21,6 +21,12 @@ Example pup_to_2_ceval :
       X 2) Y 0) Y 2) X 1) Y 3) X 0.
 Proof.
   unfold pup_to_n. apply E_Seq with (st':= update (update empty_state X 2) Y 0).
+  - apply E_Ass. simpl. reflexivity.
+  - apply E_WhileLoop with (st' := (update (update (update (update empty_state X 2) Y 0) Y 2) X 1)).
+    + simpl.
+  
+
+  unfold pup_to_n. 
   - 
 
 Qed.
